src/core/DY.Core.Trace.State.Aux.fst
@@ -5,6 +5,8 @@ open DY.Core.Bytes
 open DY.Core.Label.Type
 open DY.Core.Trace.Type
 
+module List = FStar.List.Tot.Base
+
 /// This module defines helper functions for state handling on traces.
 /// The functions will be used in `DY.Core.Trace.Invariant`
 /// to define the trace invariant
@@ -19,7 +21,7 @@ type full_state_raw = list (state_id * session_raw)
 //TODO: full_state_raw should be `Map state_id session_raw`, can we extract the generic Map part from DY.Lib.State.Map?
 // or is it not worth the effort?
 
-val max: int -> int -> int
+val max: nat -> nat -> nat
 let max x y =
   if x < y then y else x
 
@@ -31,31 +33,29 @@ val compute_new_session_id: principal -> trace -> state_id
 let rec compute_new_session_id prin tr =
   match tr with
   | Nil -> {the_id = 0}
-  | Snoc tr_init evt -> (
-    match evt with
-    | SetState prin' sess_id _ ->
+  | Snoc tr_init (SetState prin' sess_id _) ->
       if prin = prin' then
         {the_id = 
              max (sess_id.the_id + 1) (compute_new_session_id prin tr_init).the_id}
       else
         compute_new_session_id prin tr_init
-    | _ -> compute_new_session_id prin tr_init
-  )
+  | Snoc tr_init _ -> compute_new_session_id prin tr_init
+  
 
 // Sanity check
-val compute_new_session_id_correct:
+val compute_new_session_id_larger_than_id_on_trace:
   prin:principal -> tr:trace ->
   sess_id:state_id -> state_content:bytes ->
   Lemma
   (requires event_exists tr (SetState prin sess_id state_content))
   (ensures sess_id.the_id < (compute_new_session_id prin tr).the_id)
-let rec compute_new_session_id_correct prin tr sess_id state_content =
+let rec compute_new_session_id_larger_than_id_on_trace prin tr sess_id state_content =
   match tr with
   | Nil -> ()
   | Snoc tr_init evt -> (
     if evt = SetState prin sess_id state_content then ()
     else (
-      compute_new_session_id_correct prin tr_init sess_id state_content
+      compute_new_session_id_larger_than_id_on_trace prin tr_init sess_id state_content
     )
   )
 
@@ -101,45 +101,177 @@ let _ =
 
 
 /// Helper function for `get_full_state`
- 
-val append_to: #a:eqtype -> #b:Type -> list (a * rev_list b) -> a -> b -> list (a * rev_list b)
-let append_to xys key elem =
+
+val prepend: #a:Type -> x:a -> rev_list a -> rev_list a
+let rec prepend x xs =
+  match xs with
+  | Nil -> Snoc Nil x
+  | Snoc init last -> Snoc (prepend x init) last
+
+let _ =
+  let xs = Snoc (Snoc Nil 1) 2 in
+  assert( 5 `prepend` xs = Snoc (Snoc (Snoc Nil 5) 1) 2)
+
+val prepend_to: #a:eqtype -> #b:Type -> list (a * rev_list b) -> a -> b -> list (a * rev_list b)
+let prepend_to xys key elem =
   let (key_elems,rest) = FStar.List.Tot.Base.partition (fun (x, _) -> x = key) xys in
   let new_key_elems = 
     match key_elems with
     | [] -> Snoc Nil elem
-    | Cons (k,elems) _ -> Snoc elems elem
+    | Cons (k,elems) _ -> elem `prepend` elems
     in
   (key, new_key_elems) :: rest // re-ordering shouldn't matter, since key is attached to elements
 
 let _ = 
   let xs = [(1, Snoc Nil 5); (5, Nil)] in
-  assert(append_to xs 5 7 = [(5, Snoc Nil 7); (1, Snoc Nil 5)])
+  assert(prepend_to xs 5 7 = [(5, Snoc Nil 7); (1, Snoc Nil 5)]);
+  assert(prepend_to xs 1 7 = [(1, Snoc (Snoc Nil 7) 5); (5,  Nil)]);
+  assert(prepend_to xs 3 7 = [(3, Snoc Nil 7); (1, Snoc Nil 5); (5, Nil)])
 
-val get_full_state_aux: principal -> trace -> full_state_raw -> full_state_raw
-let rec get_full_state_aux prin tr curr_state =
+
+val get_full_state_aux_: principal -> trace -> full_state_raw -> full_state_raw
+let rec get_full_state_aux_ prin tr curr_state =
   match tr with
   | Nil -> curr_state
   | Snoc init (SetState p' sid' content) ->
       if p' = prin 
         then begin
-          let new_state = append_to curr_state sid' content in
-          get_full_state_aux prin init new_state
+          let new_state = prepend_to curr_state sid' content in
+          get_full_state_aux_ prin init new_state
         end
-        else get_full_state_aux prin init curr_state
-  | Snoc init _ -> get_full_state_aux prin init curr_state
+        else get_full_state_aux_ prin init curr_state
+  | Snoc init _ -> get_full_state_aux_ prin init curr_state
 
-val get_full_state: principal -> trace -> option full_state_raw
-let get_full_state prin tr = 
+val get_full_state_: principal -> trace -> option full_state_raw
+let get_full_state_ prin tr = 
   let next_state_id = compute_new_session_id prin tr in
   if next_state_id.the_id = 0
     then None
     else begin
       let full_state_init = [] in
-      match get_full_state_aux prin tr full_state_init with
+      match get_full_state_aux_ prin tr full_state_init with
       | [] -> None
       | fst -> Some fst
     end
+
+val fold_right_reverse_list:
+  ('a -> 'b -> Tot 'b) -> xs:rev_list 'a -> 'b -> Tot 'b (decreases xs)
+let rec fold_right_reverse_list f xs y =
+  match xs with 
+  | Nil -> y
+  | Snoc init x -> f x (fold_right_reverse_list f init y) // fold_right_reverse_list f (f y x) init
+
+#push-options "--fuel 4"
+let _ =
+  let xs = Snoc (Snoc Nil 3) 5 in
+  assert(fold_right_reverse_list (+) xs 0 = 8);
+  assert(fold_right_reverse_list (Cons) xs [] = [5;3]);
+  // let ys = Nil in
+  // assert(fold_right_reverse_list (fun next old -> next ^ old) "begin" ys = "begin");
+  // let ys' = Snoc Nil "a" in
+  // assert(fold_right_reverse_list (^) ys' "begin" = "abegin");
+  ()
+
+let rec state_was_set_get_session_some (p:principal) (sid:state_id) (cont:bytes) (tr:trace) :
+  Lemma 
+  (requires
+    state_was_set tr p sid cont
+  )
+  (ensures
+    Some? (get_session p sid tr)
+  )
+  //[SMTPat (state_was_set tr p sid cont)]
+  = 
+    match tr with
+    | Nil -> ()
+    | Snoc init (SetState p' sid' cont') -> 
+        if p' = p && sid' = sid
+          then ()
+          else state_was_set_get_session_some p sid cont init
+    | Snoc init _ -> state_was_set_get_session_some p sid cont init
+  
+// this is not the most efficient way to collect the full state
+// (since it goes through the trace for every new session id)
+// but this way makes it easier to prove relations of get_full_state and get_session
+val get_full_state_aux_step: principal -> tr:trace  -> full_state_raw -> ev:trace_event{event_exists tr ev} -> full_state_raw
+let get_full_state_aux_step prin tr curr_state ev =
+  match ev with
+  | (SetState p' sid' content) ->
+      if p' = prin  
+        then begin
+          if sid' `List.mem` (List.map fst curr_state)
+            then curr_state
+            else begin 
+              state_was_set_get_session_some prin sid' content tr;
+              let Some sess = get_session prin sid' tr in
+              let new_state = (sid', sess) :: curr_state in
+              new_state
+            end
+        end
+        else curr_state
+  | _ -> curr_state
+
+
+val get_full_state_aux: principal -> trace -> full_state_raw
+let get_full_state_aux prin tr =
+  assume(has_type tr (rev_list (ev:trace_event {event_exists tr ev})));
+  fold_right_reverse_list (fun ev curr_state -> get_full_state_aux_step prin tr curr_state ev) tr []
+//   match tr with
+//   | Nil -> curr_state
+//   | Snoc init (SetState p' sid' content) ->
+//       if p' = prin  
+//         then begin
+//           if sid' `List.mem` (List.map fst curr_state)
+//             then get_full_state_aux prin init curr_state
+//             else begin 
+//               let Some sess = get_session prin sid' tr in
+//               let new_state = (sid', sess) :: curr_state in
+//               get_full_state_aux prin init new_state
+//             end
+//         end
+//         else get_full_state_aux prin init curr_state
+//   | Snoc init _ -> get_full_state_aux prin init curr_state
+
+
+// val get_full_state: principal -> trace -> option full_state_raw
+// let get_full_state prin tr = 
+//       match get_full_state_aux prin tr with
+//       | [] -> None
+//       | fst -> Some fst
+
+let rec one_to (n:nat{n >= 1}) :list nat = 
+  if n = 1
+  then [1]
+  else (one_to (n-1)) @ [n]
+
+let rec zero_to_sid (sid:state_id) : 
+  Tot (list state_id ) 
+  (decreases (sid.the_id))
+  =
+  if sid.the_id = 0
+  then [{the_id = 0}]
+  else (zero_to_sid {the_id = sid.the_id - 1}) @ [sid]
+
+let get_session_list (tr:trace) (prin:principal) (sid:state_id) =
+  let session = get_session prin sid tr in
+        if Some? session
+        then [(sid,Some?.v session)]
+        else []
+
+val get_full_state: principal -> trace -> option full_state_raw
+let get_full_state prin tr = 
+  let new_sessid = compute_new_session_id prin tr in
+  if new_sessid.the_id = 0
+  then None
+  else (
+    // let sessions = List.concatMap 
+    //   (fun sid -> (
+    //     get_session_list tr prin sid)) 
+    //   (zero_to_sid new_sessid) in
+    Some (List.concatMap 
+      (get_session_list tr prin) 
+      (zero_to_sid new_sessid))
+  )
 
 // tests for `get_full_state`
 let _ =
@@ -147,8 +279,21 @@ let _ =
   let sid1 = {the_id = 1} in
   let sid2 = {the_id = 2} in
   let b = Literal (FStar.Seq.Base.empty) in
-  let tr = Snoc (Snoc Nil (SetState p sid1 b)) (SetState p sid2 b) in
-  assert(get_full_state p tr = Some [(sid1, (Snoc Nil b)); (sid2, Snoc Nil b)]);
+  let b1 = Literal (FStar.Seq.Base.create 1 FStar.UInt8.one ) in
+  let tr = Snoc ( Snoc (Snoc Nil (SetState p sid1 b)) (SetState p sid2 b) ) (SetState p sid1 b1) in
+  assert(get_session p sid1 tr =  Some (Snoc (Snoc Nil b) b1));
+  assert(get_session p sid2 tr = Some (Snoc Nil b));
+  assert(compute_new_session_id p tr = {the_id = 3});
+  assert(zero_to_sid {the_id = 3} = [ {the_id = 0}; sid1; sid2; {the_id = 3} ]);
+//  assert(None? (get_session p {the_id = 0} tr));
+//  assert(None? (get_session p {the_id = 3} tr));
+  assert((List.concatMap (get_session_list tr p) [sid1; sid2])
+  = [(sid1, Snoc (Snoc Nil b) b1); (sid2, Snoc Nil b) ]
+  );
+  // assert((List.concatMap (get_session_list tr p) [{the_id = 0}; sid1; sid2; {the_id = 3}])
+  // = [(sid1, Snoc (Snoc Nil b) b1); (sid2, Snoc Nil b) ]
+  // );
+  assert(get_full_state p tr = Some [(sid1, Snoc (Snoc Nil b) b1); (sid2, Snoc Nil b); ]);
   assert(None? (get_full_state "b" tr))
 
 
